Weidenbach_Book/CDCL_Two_Watched_Literals_List_Watched_Init_Trail_Code.thy
@@ -51,7 +51,7 @@ proof -
     finalise_init_finalise_init] unfolding PR_CONST_def .
   have pre: \<open>?pre' x\<close> if \<open>?pre x\<close> for x
     using that by (auto simp: comp_PRE_def twl_st_trail_ref_def trailt_ref_def option_conflict_rel_def
-        conflict_rel_def in_N\<^sub>1_atm_of_in_atms_of_iff)
+        conflict_rel_def in_\<L>\<^sub>a\<^sub>l\<^sub>l_atm_of_in_atms_of_iff)
 
   have im: \<open>?im' = ?im\<close> and f: \<open>?f' = ?f\<close>
     unfolding prod_hrp_comp hrp_comp_dest hrp_comp_keep conflict_option_assn_def
@@ -96,7 +96,7 @@ concrete_definition (in -) propagate_unit_cls_code
 prepare_code_thms (in -) propagate_unit_cls_code_def
 
 lemmas propagate_unit_cls_int_hnr[sepref_fr_rules] =
-   propagate_unit_cls_code.refine[of N\<^sub>0, OF twl_array_code_axioms]
+   propagate_unit_cls_code.refine[of \<A>\<^sub>i\<^sub>n, OF twl_array_code_axioms]
 
 theorem propagate_unit_cls_hnr[sepref_fr_rules]:
   \<open>(uncurry propagate_unit_cls_code, uncurry (RETURN oo propagate_unit_cls))
@@ -163,7 +163,7 @@ concrete_definition (in -) already_propagated_unit_cls_code
 prepare_code_thms (in -) already_propagated_unit_cls_code_def
 
 lemmas already_propagated_unit_cls_int_hnr[sepref_fr_rules] =
-   already_propagated_unit_cls_code.refine[of N\<^sub>0, OF twl_array_code_axioms]
+   already_propagated_unit_cls_code.refine[of \<A>\<^sub>i\<^sub>n, OF twl_array_code_axioms]
 
 theorem already_propagated_unit_cls_hnr[sepref_fr_rules]:
   \<open>(uncurry already_propagated_unit_cls_code, uncurry (RETURN \<circ>\<circ> already_propagated_unit_cls))
@@ -199,7 +199,7 @@ lemma set_conflict_unit_int_set_conflict_unit:
      \<langle>option_conflict_rel\<rangle>nres_rel\<close>
   by (intro frefI nres_relI)
     (auto simp: twl_st_ref_def set_conflict_unit_int_def set_conflict_unit_def
-      option_conflict_rel_def conflict_rel_def in_N\<^sub>1_atm_of_in_atms_of_iff
+      option_conflict_rel_def conflict_rel_def in_\<L>\<^sub>a\<^sub>l\<^sub>l_atm_of_in_atms_of_iff
       intro!: mset_as_position.intros)
 
 sepref_thm set_conflict_unit_code
@@ -217,7 +217,7 @@ concrete_definition (in -) set_conflict_unit_code
 prepare_code_thms (in -) set_conflict_unit_code_def
 
 lemmas set_conflict_unit_int_hnr[sepref_fr_rules] =
-   set_conflict_unit_code.refine[of N\<^sub>0, OF twl_array_code_axioms]
+   set_conflict_unit_code.refine[of \<A>\<^sub>i\<^sub>n, OF twl_array_code_axioms]
 
 theorem set_conflict_unit_hnr[sepref_fr_rules]:
   \<open>(uncurry set_conflict_unit_code, uncurry (RETURN oo set_conflict_unit))
@@ -241,7 +241,7 @@ proof -
     set_conflict_unit_int_set_conflict_unit] .
   have pre: \<open>?pre' x\<close> if \<open>?pre x\<close> for x
     using that by (auto simp: comp_PRE_def option_conflict_rel_def conflict_rel_def image_image
-        in_N\<^sub>1_atm_of_in_atms_of_iff)
+        in_\<L>\<^sub>a\<^sub>l\<^sub>l_atm_of_in_atms_of_iff)
   have im: \<open>?im' = ?im\<close>
     unfolding prod_hrp_comp hrp_comp_dest hrp_comp_keep conflict_option_assn_def by simp
   have f: \<open>?f' = ?f\<close>
@@ -271,7 +271,7 @@ concrete_definition (in -) conflict_propagated_unit_cls_code
 prepare_code_thms (in -) conflict_propagated_unit_cls_code_def
 
 lemmas conflict_propagated_unit_cls_int_hnr[sepref_fr_rules] =
-   conflict_propagated_unit_cls_code.refine[of N\<^sub>0, OF twl_array_code_axioms]
+   conflict_propagated_unit_cls_code.refine[of \<A>\<^sub>i\<^sub>n, OF twl_array_code_axioms]
 
 theorem conflict_propagated_unit_cls_hnr[sepref_fr_rules]:
   \<open>(uncurry conflict_propagated_unit_cls_code, uncurry (RETURN oo conflict_propagated_unit_cls))
@@ -342,11 +342,11 @@ concrete_definition (in -) add_init_cls_code
 prepare_code_thms (in -) add_init_cls_code_def
 
 lemmas add_init_cls_int_hnr[sepref_fr_rules] =
-   add_init_cls_code.refine[of N\<^sub>0, OF twl_array_code_axioms]
+   add_init_cls_code.refine[of \<A>\<^sub>i\<^sub>n, OF twl_array_code_axioms]
 
 lemma add_init_cls_int_add_init_cls:
   \<open>(uncurry add_init_cls_int, uncurry (add_init_cls)) \<in>
-   [\<lambda>(C, S). length C \<ge> 2 \<and> literals_are_in_N\<^sub>0 (mset C)]\<^sub>f
+   [\<lambda>(C, S). length C \<ge> 2 \<and> literals_are_in_\<A>\<^sub>i\<^sub>n (mset C)]\<^sub>f
    Id \<times>\<^sub>r twl_st_ref_no_clvls \<rightarrow> \<langle>twl_st_ref_no_clvls\<rangle> nres_rel\<close>
   by (intro frefI nres_relI)
     (auto simp: twl_st_ref_no_clvls_def add_init_cls_int_def add_init_cls_def Let_def
@@ -354,14 +354,14 @@ lemma add_init_cls_int_add_init_cls:
 
 theorem add_init_cls_hnr[sepref_fr_rules]:
   \<open>(uncurry add_init_cls_code, uncurry add_init_cls)
-    \<in> [\<lambda>(C, S). length C \<ge> 2 \<and> literals_are_in_N\<^sub>0 (mset C)]\<^sub>a
+    \<in> [\<lambda>(C, S). length C \<ge> 2 \<and> literals_are_in_\<A>\<^sub>i\<^sub>n (mset C)]\<^sub>a
       (list_assn unat_lit_assn)\<^sup>k *\<^sub>a twl_st_assn_no_clvls\<^sup>d  \<rightarrow> twl_st_assn_no_clvls\<close>
     (is \<open>?c \<in> [?pre]\<^sub>a ?im \<rightarrow> ?f\<close>)
 proof -
   have H: \<open>?c
     \<in> [comp_PRE (Id \<times>\<^sub>f twl_st_ref_no_clvls)
      (\<lambda>(C, S).
-         2 \<le> length C \<and> literals_are_in_N\<^sub>0 (mset C))
+         2 \<le> length C \<and> literals_are_in_\<A>\<^sub>i\<^sub>n (mset C))
      (\<lambda>_ (C, S).
          C \<noteq> [] \<and>
          tl C \<noteq> [] \<and>
@@ -381,7 +381,7 @@ proof -
   have pre: \<open>?pre' x\<close> if \<open>?pre x\<close> for x
     apply (cases \<open>fst x\<close>; cases \<open>tl (fst x)\<close>)
     using that by (auto simp: comp_PRE_def twl_st_ref_no_clvls_def image_image map_fun_rel_def
-        literals_are_in_N\<^sub>0_add_mset)
+        literals_are_in_\<A>\<^sub>i\<^sub>n_add_mset)
   have im: \<open>?im' = ?im\<close>
     unfolding prod_hrp_comp hrp_comp_dest hrp_comp_keep twl_st_assn_no_clvls_def by simp
   have f: \<open>?f' = ?f\<close>
@@ -431,7 +431,7 @@ concrete_definition (in -) already_propagated_unit_cls_conflict_code
 prepare_code_thms (in -) already_propagated_unit_cls_conflict_code_def
 
 lemmas already_propagated_unit_cls_conflict_int_hnr[sepref_fr_rules] =
-   already_propagated_unit_cls_conflict_code.refine[of N\<^sub>0, OF twl_array_code_axioms]
+   already_propagated_unit_cls_conflict_code.refine[of \<A>\<^sub>i\<^sub>n, OF twl_array_code_axioms]
 
 lemma already_propagated_unit_cls_conflict_hnr[sepref_fr_rules]:
   \<open>(uncurry already_propagated_unit_cls_conflict_code,
@@ -460,7 +460,7 @@ definition init_dt_step_wl :: \<open>nat clause_l \<Rightarrow> nat twl_st_wl \<
            }
          else do {
           ASSERT(length C \<ge> 2);
-          ASSERT(literals_are_in_N\<^sub>0 (mset C));
+          ASSERT(literals_are_in_\<A>\<^sub>i\<^sub>n (mset C));
           add_init_cls C S}}
     else do {
         if length C = 1
@@ -471,7 +471,7 @@ definition init_dt_step_wl :: \<open>nat clause_l \<Rightarrow> nat twl_st_wl \<
         else do {
           ASSERT(hd C \<in> snd ` D\<^sub>0);
           ASSERT(length C \<ge> 2);
-          ASSERT(literals_are_in_N\<^sub>0 (mset C));
+          ASSERT(literals_are_in_\<A>\<^sub>i\<^sub>n (mset C));
           add_init_cls C S}}
   }\<close>
 
@@ -636,7 +636,7 @@ lemma in_map_atm_of_hnr[sepref_fr_rules]:
 
 
 definition extract_atms_cls :: \<open>'a clause_l \<Rightarrow> 'a list \<Rightarrow> 'a list\<close> where
-  \<open>extract_atms_cls C N\<^sub>0 = fold (\<lambda>L N\<^sub>0. if atm_of L \<in> set N\<^sub>0 then N\<^sub>0 else atm_of L # N\<^sub>0) C N\<^sub>0\<close>
+  \<open>extract_atms_cls C \<A>\<^sub>i\<^sub>n = fold (\<lambda>L \<A>\<^sub>i\<^sub>n. if atm_of L \<in> set \<A>\<^sub>i\<^sub>n then \<A>\<^sub>i\<^sub>n else atm_of L # \<A>\<^sub>i\<^sub>n) C \<A>\<^sub>i\<^sub>n\<close>
 
 sepref_definition extract_atms_cls_imp
   is \<open>uncurry (RETURN oo extract_atms_cls)\<close>
@@ -647,7 +647,7 @@ sepref_definition extract_atms_cls_imp
 declare extract_atms_cls_imp.refine[sepref_fr_rules]
 
 definition extract_atms_clss:: \<open>'a clauses_l \<Rightarrow> 'a list \<Rightarrow> 'a list\<close>  where
-  \<open>extract_atms_clss N N\<^sub>0 = fold extract_atms_cls N N\<^sub>0\<close>
+  \<open>extract_atms_clss N \<A>\<^sub>i\<^sub>n = fold extract_atms_cls N \<A>\<^sub>i\<^sub>n\<close>
 
 sepref_definition extract_atms_clss_imp
   is \<open>uncurry (RETURN oo extract_atms_clss)\<close>
@@ -694,7 +694,7 @@ sepref_definition find_first_eq_map_atm_of_code
   by sepref
 
 definition index_atm_of where
-  \<open>index_atm_of L N\<^sub>0 = index (map atm_of N\<^sub>0) L\<close>
+  \<open>index_atm_of L \<A>\<^sub>i\<^sub>n = index (map atm_of \<A>\<^sub>i\<^sub>n) L\<close>
 
 lemma find_first_eq_map_atm_of_code_index_atm_of[sepref_fr_rules]:
   \<open>(uncurry find_first_eq_map_atm_of_code, uncurry (RETURN oo index_atm_of)) \<in>
@@ -709,11 +709,11 @@ proof -
 qed
 
 lemma extract_atms_cls_Cons:
-  \<open>extract_atms_cls (L # C) N\<^sub>0 = extract_atms_cls C (if atm_of L \<in> set N\<^sub>0 then N\<^sub>0 else atm_of L # N\<^sub>0)\<close>
+  \<open>extract_atms_cls (L # C) \<A>\<^sub>i\<^sub>n = extract_atms_cls C (if atm_of L \<in> set \<A>\<^sub>i\<^sub>n then \<A>\<^sub>i\<^sub>n else atm_of L # \<A>\<^sub>i\<^sub>n)\<close>
   unfolding extract_atms_cls_def fold.simps by simp
 
 lemma extract_atms_cls_Nil[simp]:
-  \<open>extract_atms_cls [] N\<^sub>0 = N\<^sub>0\<close>
+  \<open>extract_atms_cls [] \<A>\<^sub>i\<^sub>n = \<A>\<^sub>i\<^sub>n\<close>
   unfolding extract_atms_cls_def fold.simps by simp
 
 lemma extract_atms_clss_Cons[simp]:
@@ -753,9 +753,9 @@ lemma all_lits_of_atms_m_all_lits_of_m:
   unfolding all_lits_of_atms_m_def all_lits_of_m_def
   by (induction N) auto
 
-lemma all_lits_of_m_extract_atms_cls: \<open>set_mset (all_lits_of_atms_m (mset (extract_atms_cls C N\<^sub>0))) =
-   set_mset (all_lits_of_m (mset C) + all_lits_of_atms_m (mset N\<^sub>0))\<close>
-  apply (induction C arbitrary: N\<^sub>0)
+lemma all_lits_of_m_extract_atms_cls: \<open>set_mset (all_lits_of_atms_m (mset (extract_atms_cls C \<A>\<^sub>i\<^sub>n))) =
+   set_mset (all_lits_of_m (mset C) + all_lits_of_atms_m (mset \<A>\<^sub>i\<^sub>n))\<close>
+  apply (induction C arbitrary: \<A>\<^sub>i\<^sub>n)
   subgoal by simp
   subgoal by (auto simp add: extract_atms_cls_Cons all_lits_of_m_add_mset uminus_literal_def
         in_all_lits_of_m_ain_atms_of_iff insert_absorb all_lits_of_atms_m_all_lits_of_m)
@@ -766,64 +766,64 @@ lemma nat_of_lit_upperN_nat_of_lit_uminus_upperN:
   by (cases L) (auto simp: upperN_def)
 
 lemma in_extract_atms_clsD:
-  \<open>set (extract_atms_cls C N\<^sub>0) = atms_of_s (set C) \<union> set N\<^sub>0\<close>
-  apply (induction C arbitrary: N\<^sub>0)
+  \<open>set (extract_atms_cls C \<A>\<^sub>i\<^sub>n) = atms_of_s (set C) \<union> set \<A>\<^sub>i\<^sub>n\<close>
+  apply (induction C arbitrary: \<A>\<^sub>i\<^sub>n)
   subgoal by auto
-  subgoal premises IH for L' C N\<^sub>0
-    using IH(1)[of \<open>(if atm_of L' \<in> set N\<^sub>0 then N\<^sub>0 else atm_of L' # N\<^sub>0)\<close>]
+  subgoal premises IH for L' C \<A>\<^sub>i\<^sub>n
+    using IH(1)[of \<open>(if atm_of L' \<in> set \<A>\<^sub>i\<^sub>n then \<A>\<^sub>i\<^sub>n else atm_of L' # \<A>\<^sub>i\<^sub>n)\<close>]
     by (auto simp: extract_atms_cls_def split: if_splits)
   done
 
 lemma in_extract_atms_clssD:
-  fixes N\<^sub>0 :: \<open>'a list\<close>
+  fixes \<A>\<^sub>i\<^sub>n :: \<open>'a list\<close>
   shows
-    \<open>set (extract_atms_clss C N\<^sub>0) = atms_of_s (\<Union>(set`set C)) \<union> set N\<^sub>0\<close>
-  apply (induction C arbitrary: N\<^sub>0)
+    \<open>set (extract_atms_clss C \<A>\<^sub>i\<^sub>n) = atms_of_s (\<Union>(set`set C)) \<union> set \<A>\<^sub>i\<^sub>n\<close>
+  apply (induction C arbitrary: \<A>\<^sub>i\<^sub>n)
   subgoal by (auto simp: extract_atms_clss_def)
-  subgoal premises IH for L' C N\<^sub>0
-    using IH(1)[of \<open>extract_atms_cls L' N\<^sub>0\<close>]
+  subgoal premises IH for L' C \<A>\<^sub>i\<^sub>n
+    using IH(1)[of \<open>extract_atms_cls L' \<A>\<^sub>i\<^sub>n\<close>]
     by (auto simp: extract_atms_clss_def in_extract_atms_clsD split: if_splits)
   done
 
-lemma is_N\<^sub>1_extract_atms_clss:
-  assumes upper: \<open>\<forall>L \<in> set N\<^sub>0. L < upperN div 2\<close>
+lemma is_\<L>\<^sub>a\<^sub>l\<^sub>l_extract_atms_clss:
+  assumes upper: \<open>\<forall>L \<in> set \<A>\<^sub>i\<^sub>n. L < upperN div 2\<close>
   assumes upperN: \<open>\<forall>C \<in> set N. \<forall>L \<in> set C. nat_of_lit L < upperN\<close>
   shows
-   \<open>twl_array_code_ops.is_N\<^sub>1 (mset (extract_atms_clss N N\<^sub>0))
-     (all_lits_of_mm (mset `# mset N) + all_lits_of_atms_m (mset N\<^sub>0))\<close>
+   \<open>twl_array_code_ops.is_\<L>\<^sub>a\<^sub>l\<^sub>l (mset (extract_atms_clss N \<A>\<^sub>i\<^sub>n))
+     (all_lits_of_mm (mset `# mset N) + all_lits_of_atms_m (mset \<A>\<^sub>i\<^sub>n))\<close>
 proof -
-  have atm_of_N\<^sub>0_iff: \<open>atm_of x \<in> set N\<^sub>0 \<longleftrightarrow>
-         x \<in> (- literal_of_nat \<circ>\<circ> op *) 2 ` set N\<^sub>0 \<or> x \<in> (literal_of_nat \<circ>\<circ> op *) 2 ` set N\<^sub>0\<close>
-    for x N\<^sub>0
+  have atm_of_\<A>\<^sub>i\<^sub>n_iff: \<open>atm_of x \<in> set \<A>\<^sub>i\<^sub>n \<longleftrightarrow>
+         x \<in> (- literal_of_nat \<circ>\<circ> op *) 2 ` set \<A>\<^sub>i\<^sub>n \<or> x \<in> (literal_of_nat \<circ>\<circ> op *) 2 ` set \<A>\<^sub>i\<^sub>n\<close>
+    for x \<A>\<^sub>i\<^sub>n
     by (cases x) auto
-  have is_N\<^sub>1_add: \<open>twl_array_code_ops.is_N\<^sub>1 N\<^sub>0 (A + B) \<longleftrightarrow> set_mset A \<subseteq> set_mset (twl_array_code_ops.N\<^sub>1 N\<^sub>0)\<close>
-    if \<open>twl_array_code_ops.is_N\<^sub>1 N\<^sub>0 B\<close> for A B N\<^sub>0
-    using that unfolding twl_array_code_ops.is_N\<^sub>1_def by auto
-  have H1: \<open>xa \<in> set N\<^sub>0 \<Longrightarrow> literal_of_nat (2 * xa) \<in> Pos ` set N\<^sub>0\<close> for xa N\<^sub>0
+  have is_\<L>\<^sub>a\<^sub>l\<^sub>l_add: \<open>twl_array_code_ops.is_\<L>\<^sub>a\<^sub>l\<^sub>l \<A>\<^sub>i\<^sub>n (A + B) \<longleftrightarrow> set_mset A \<subseteq> set_mset (twl_array_code_ops.\<L>\<^sub>a\<^sub>l\<^sub>l \<A>\<^sub>i\<^sub>n)\<close>
+    if \<open>twl_array_code_ops.is_\<L>\<^sub>a\<^sub>l\<^sub>l \<A>\<^sub>i\<^sub>n B\<close> for A B \<A>\<^sub>i\<^sub>n
+    using that unfolding twl_array_code_ops.is_\<L>\<^sub>a\<^sub>l\<^sub>l_def by auto
+  have H1: \<open>xa \<in> set \<A>\<^sub>i\<^sub>n \<Longrightarrow> literal_of_nat (2 * xa) \<in> Pos ` set \<A>\<^sub>i\<^sub>n\<close> for xa \<A>\<^sub>i\<^sub>n
     by auto
-  have H2: \<open>xa \<in> set N\<^sub>0 \<Longrightarrow> - literal_of_nat (2 * xa) \<in> Neg ` set N\<^sub>0\<close> for xa N\<^sub>0
+  have H2: \<open>xa \<in> set \<A>\<^sub>i\<^sub>n \<Longrightarrow> - literal_of_nat (2 * xa) \<in> Neg ` set \<A>\<^sub>i\<^sub>n\<close> for xa \<A>\<^sub>i\<^sub>n
     by auto
   show ?thesis
     using upper upperN
-  proof (induction N arbitrary: N\<^sub>0)
+  proof (induction N arbitrary: \<A>\<^sub>i\<^sub>n)
     case Nil
     then show ?case
       using H1 H2
-      by (auto simp: extract_atms_cls_def extract_atms_clss_def twl_array_code_ops.is_N\<^sub>1_def
-          twl_array_code_ops.N\<^sub>1_def in_all_lits_of_m_ain_atms_of_iff
+      by (auto simp: extract_atms_cls_def extract_atms_clss_def twl_array_code_ops.is_\<L>\<^sub>a\<^sub>l\<^sub>l_def
+          twl_array_code_ops.\<L>\<^sub>a\<^sub>l\<^sub>l_def in_all_lits_of_m_ain_atms_of_iff
           atm_of_eq_atm_of all_lits_of_atms_m_all_lits_of_m
-          atm_of_N\<^sub>0_iff
+          atm_of_\<A>\<^sub>i\<^sub>n_iff
           simp del: nat_of_lit.simps literal_of_nat.simps)
   next
-    case (Cons C Cs N\<^sub>0) note IH = this(1) and H=this(2-)
+    case (Cons C Cs \<A>\<^sub>i\<^sub>n) note IH = this(1) and H=this(2-)
     have \<open>2 * L < upperN \<longleftrightarrow> L < upperN div 2\<close> for L
       by (auto simp: upperN_def)
-    then have \<open>\<forall>L\<in>set (extract_atms_cls C N\<^sub>0). L < upperN div 2\<close>
+    then have \<open>\<forall>L\<in>set (extract_atms_cls C \<A>\<^sub>i\<^sub>n). L < upperN div 2\<close>
       using Cons
       by (auto simp: in_extract_atms_clsD nat_of_lit_upperN_nat_of_lit_uminus_upperN)
     then show ?case
-      using IH[of \<open>extract_atms_cls C N\<^sub>0\<close>, unfolded twl_array_code_ops.is_N\<^sub>1_def] H
-      by (simp add: all_lits_of_mm_add_mset twl_array_code_ops.is_N\<^sub>1_def
+      using IH[of \<open>extract_atms_cls C \<A>\<^sub>i\<^sub>n\<close>, unfolded twl_array_code_ops.is_\<L>\<^sub>a\<^sub>l\<^sub>l_def] H
+      by (simp add: all_lits_of_mm_add_mset twl_array_code_ops.is_\<L>\<^sub>a\<^sub>l\<^sub>l_def
           all_lits_of_m_extract_atms_cls ac_simps comp_def)
   qed
 qed
@@ -834,7 +834,7 @@ begin
 
 fun correct_watching_init :: \<open>nat twl_st_wl \<Rightarrow> bool\<close> where
   \<open>correct_watching_init (M, N, U, D, NP, UP, Q, W) \<longleftrightarrow>
-    (\<forall>L \<in># all_lits_of_atms_m N\<^sub>0. mset (W L) = clause_to_update L (M, N, U, D, NP, UP, {#}, {#}))\<close>
+    (\<forall>L \<in># all_lits_of_atms_m \<A>\<^sub>i\<^sub>n. mset (W L) = clause_to_update L (M, N, U, D, NP, UP, {#}, {#}))\<close>
 
 
 lemma clause_to_update_append: \<open>N \<noteq> [] \<Longrightarrow> clause_to_update La (M, N @ [C], U, D, NP, UP, WS, Q) =
@@ -848,22 +848,22 @@ definition HH :: \<open>(nat twl_st_wl \<times> nat twl_st_l) set\<close> where
                M = M' \<and> N = N' \<and> U = U' \<and> D = D' \<and> NP = NP' \<and> UP = UP' \<and> Q = Q' \<and> WS = {#} \<and>
                (* U = length N - 1 \<and> *) UP = {#} \<and> N \<noteq> [] \<and>
                correct_watching_init (M', N', U', D', NP', UP', Q', WS') \<and>
-               set_mset (all_lits_of_mm (mset `# mset (tl N) + NP)) \<subseteq> set_mset N\<^sub>1 \<and>
+               set_mset (all_lits_of_mm (mset `# mset (tl N) + NP)) \<subseteq> set_mset \<L>\<^sub>a\<^sub>l\<^sub>l \<and>
                (\<forall>L \<in> lits_of_l M. {#L#} \<in># NP) \<and>
                (\<forall>L \<in> set M. \<exists>K. L = Propagated K 0) \<and>
                (D \<noteq> None \<longrightarrow> Q = {#})}\<close>
 
 
-lemma literals_are_in_N\<^sub>0_add_mset:
-  \<open>literals_are_in_N\<^sub>0 (add_mset L M) \<longleftrightarrow> literals_are_in_N\<^sub>0 M \<and> atm_of L \<in># N\<^sub>0\<close>
+lemma literals_are_in_\<A>\<^sub>i\<^sub>n_add_mset:
+  \<open>literals_are_in_\<A>\<^sub>i\<^sub>n (add_mset L M) \<longleftrightarrow> literals_are_in_\<A>\<^sub>i\<^sub>n M \<and> atm_of L \<in># \<A>\<^sub>i\<^sub>n\<close>
   by (cases L)
-   (auto simp: N\<^sub>1_def literals_are_in_N\<^sub>0_def image_image all_lits_of_m_add_mset uminus_lit_swap
+   (auto simp: \<L>\<^sub>a\<^sub>l\<^sub>l_def literals_are_in_\<A>\<^sub>i\<^sub>n_def image_image all_lits_of_m_add_mset uminus_lit_swap
          simp del: literal_of_nat.simps)
 
 lemma init_dt_step_wl_init_dt_step_l:
   assumes
     S'S: \<open>(S', S) \<in> HH\<close> and
-    lits_C: \<open>literals_are_in_N\<^sub>0 (mset C)\<close> and
+    lits_C: \<open>literals_are_in_\<A>\<^sub>i\<^sub>n (mset C)\<close> and
     dist_C: \<open>distinct C\<close>
   shows \<open>init_dt_step_wl C S' \<le> \<Down> HH (init_dt_step_l C S)\<close>
 proof -
@@ -874,28 +874,28 @@ proof -
     if \<open>N = N'\<close>
     for M N U D NP UP WS Q M' N' U' D' NP' UP' WS' Q' and L :: \<open>nat literal\<close>
     by (auto simp: clause_to_update_def that)
-  note literal_of_nat.simps[simp del] atms_of_N\<^sub>1_N\<^sub>0[simp]
-  have hd_C: \<open>hd C \<in> snd ` (\<lambda>L. (nat_of_lit L, L)) ` set_mset N\<^sub>1\<close>
-      \<open>-hd C \<in> snd ` (\<lambda>L. (nat_of_lit L, L)) ` set_mset N\<^sub>1\<close>
+  note literal_of_nat.simps[simp del] atms_of_\<L>\<^sub>a\<^sub>l\<^sub>l_\<A>\<^sub>i\<^sub>n[simp]
+  have hd_C: \<open>hd C \<in> snd ` (\<lambda>L. (nat_of_lit L, L)) ` set_mset \<L>\<^sub>a\<^sub>l\<^sub>l\<close>
+      \<open>-hd C \<in> snd ` (\<lambda>L. (nat_of_lit L, L)) ` set_mset \<L>\<^sub>a\<^sub>l\<^sub>l\<close>
     if \<open>C \<noteq> []\<close>
     using assms(3-) that lits_C
     by (cases C; cases \<open>hd C\<close>;
         auto simp: HH_def correct_watching.simps clause_to_update_def image_image
-        all_lits_of_mm_add_mset all_lits_of_m_add_mset twl_array_code_ops.N\<^sub>1_def
-        clauses_def mset_take_mset_drop_mset' literals_are_in_N\<^sub>0_add_mset)+
+        all_lits_of_mm_add_mset all_lits_of_m_add_mset twl_array_code_ops.\<L>\<^sub>a\<^sub>l\<^sub>l_def
+        clauses_def mset_take_mset_drop_mset' literals_are_in_\<A>\<^sub>i\<^sub>n_add_mset)+
 
-  have hd_tl_C: \<open>hd (tl C) \<in> snd ` (\<lambda>L. (nat_of_lit L, L)) ` set_mset (twl_array_code_ops.N\<^sub>1 N\<^sub>0)\<close>
+  have hd_tl_C: \<open>hd (tl C) \<in> snd ` (\<lambda>L. (nat_of_lit L, L)) ` set_mset (twl_array_code_ops.\<L>\<^sub>a\<^sub>l\<^sub>l \<A>\<^sub>i\<^sub>n)\<close>
     if \<open>C \<noteq> []\<close> and \<open>tl C \<noteq> []\<close>
     using assms(3-) that lits_C by (cases C; cases \<open>tl C\<close>)
       (auto simp: HH_def Let_def clause_to_update_append
         clauses_def mset_take_mset_drop_mset' image_image all_lits_of_m_add_mset
-        twl_array_code_ops.literals_are_in_N\<^sub>0_def)
+        twl_array_code_ops.literals_are_in_\<A>\<^sub>i\<^sub>n_def)
 
   obtain M N U D NP Q WS where
     S': \<open>S' = (M, N, U, D, NP, {#}, Q, WS)\<close> and
     S: \<open>S = (M, N, U, D, NP, {#}, {#}, Q)\<close> and
     H: \<open>correct_watching_init (M, N, U, D, NP, {#}, Q, WS)\<close>
-     \<open>set_mset (all_lits_of_mm (mset `# mset (tl N) + NP)) \<subseteq> set_mset N\<^sub>1\<close>
+     \<open>set_mset (all_lits_of_mm (mset `# mset (tl N) + NP)) \<subseteq> set_mset \<L>\<^sub>a\<^sub>l\<^sub>l\<close>
      \<open>\<forall>L\<in>lits_of_l M. {#L#} \<in># NP\<close>
      \<open>\<forall>L\<in>set M. \<exists>K. L = Propagated K 0\<close>
      \<open>N \<noteq> []\<close>
@@ -920,17 +920,17 @@ proof -
       \<open>C \<noteq> []\<close> and
       \<open>tl C \<noteq> []\<close> and
       C_ge2: \<open>2 \<le> length C\<close> and
-      \<open>literals_are_in_N\<^sub>0 (mset C)\<close>
+      \<open>literals_are_in_\<A>\<^sub>i\<^sub>n (mset C)\<close>
   proof -
     obtain L1 L2 C' where C: \<open>C = L1 # L2 # C'\<close>
       using C_ge2 by (cases C; cases \<open>tl C\<close>) auto
     have [simp]: \<open>L2 \<noteq> L1\<close>
       using dist unfolding C by auto
-    have \<open>set_mset (all_lits_of_mm (mset `# mset (tl (N @ [L1 # L2 # C'])) + NP)) \<subseteq> set_mset N\<^sub>1\<close>
+    have \<open>set_mset (all_lits_of_mm (mset `# mset (tl (N @ [L1 # L2 # C'])) + NP)) \<subseteq> set_mset \<L>\<^sub>a\<^sub>l\<^sub>l\<close>
       using lits_C H unfolding C
-      by (auto simp add: all_lits_of_mm_add_mset in_N\<^sub>1_atm_of_in_atms_of_iff
-          all_lits_of_m_add_mset literals_are_in_N\<^sub>0_add_mset
-          literals_are_in_N\<^sub>0_def)
+      by (auto simp add: all_lits_of_mm_add_mset in_\<L>\<^sub>a\<^sub>l\<^sub>l_atm_of_in_atms_of_iff
+          all_lits_of_m_add_mset literals_are_in_\<A>\<^sub>i\<^sub>n_add_mset
+          literals_are_in_\<A>\<^sub>i\<^sub>n_def)
     then show ?thesis
       using H
       unfolding HH_def C
@@ -950,7 +950,7 @@ proof -
       using H D lits_C
       unfolding HH_def
       by (cases C) (auto simp: clause_to_update_append all_lits_of_mm_add_mset
-          all_lits_of_m_add_mset literals_are_in_N\<^sub>0_add_mset in_N\<^sub>1_atm_of_in_atms_of_iff)
+          all_lits_of_m_add_mset literals_are_in_\<A>\<^sub>i\<^sub>n_add_mset in_\<L>\<^sub>a\<^sub>l\<^sub>l_atm_of_in_atms_of_iff)
   qed
   have le1_propa_no_confl:
     \<open>((Propagated (hd C) 0 # M, N, U, D, add_mset {#hd C#} NP,
@@ -978,7 +978,7 @@ proof -
     using H hd_C hd_tl_C dist_C C lits_C
     by (cases C; cases \<open>tl C\<close>)
       (auto simp: HH_def all_lits_of_mm_add_mset all_lits_of_m_add_mset
-        clause_to_update_append uminus_N\<^sub>0_iff literals_are_in_N\<^sub>0_def)
+        clause_to_update_append uminus_\<A>\<^sub>i\<^sub>n_iff literals_are_in_\<A>\<^sub>i\<^sub>n_def)
   have C_ge_2_iff: \<open>2 \<le> length C \<longleftrightarrow> C \<noteq> [] \<and> tl C \<noteq> []\<close>
     by (cases C; cases \<open>tl C\<close>) auto
   show ?thesis
@@ -1013,7 +1013,7 @@ qed
 lemma init_dt_wl_init_dt_l:
   assumes
     S'S: \<open>(S', S) \<in> HH\<close> and
-    \<open>\<forall>C\<in>set CS. literals_are_in_N\<^sub>0 (mset C)\<close> and
+    \<open>\<forall>C\<in>set CS. literals_are_in_\<A>\<^sub>i\<^sub>n (mset C)\<close> and
     \<open>\<forall>C\<in>set CS. distinct C\<close>
   shows \<open>init_dt_wl CS S' \<le> \<Down> HH (init_dt_l CS S)\<close>
   using assms
@@ -1046,18 +1046,18 @@ lemma init_dt_init_dt_l_full:
     stgy_invs: \<open>twl_stgy_invs (twl_st_of_wl None S)\<close> and
     watch: \<open>correct_watching_init S\<close> and
     clss: \<open>get_clauses_wl S \<noteq> []\<close> and
-    S_N\<^sub>1: \<open>set_mset (all_lits_of_mm (cdcl\<^sub>W_restart_mset.clauses
-      (state\<^sub>W_of (twl_st_of None (st_l_of_wl None S))))) \<subseteq> set_mset N\<^sub>1\<close> and
+    S_\<L>\<^sub>a\<^sub>l\<^sub>l: \<open>set_mset (all_lits_of_mm (cdcl\<^sub>W_restart_mset.clauses
+      (state\<^sub>W_of (twl_st_of None (st_l_of_wl None S))))) \<subseteq> set_mset \<L>\<^sub>a\<^sub>l\<^sub>l\<close> and
     no_learned: \<open>get_unit_learned S = {#}\<close> and
     confl_in_clss: \<open>get_conflict_wl S \<noteq> None \<longrightarrow> the (get_conflict_wl S) \<in># mset `# mset CS\<close> and
     trail_in_NP: \<open>\<forall>L \<in> lits_of_l (get_trail_wl S). {#L#} \<in># get_unit_init_clss S\<close> and
     prop_NP: \<open>\<forall>L \<in> set (get_trail_wl S). \<exists>K. L = Propagated K 0\<close> and
     upper: \<open>\<forall>C\<in>set CS. \<forall>L\<in>set C. nat_of_lit L < upperN\<close> and
-    is_N\<^sub>1: \<open>is_N\<^sub>1 (all_lits_of_mm (mset `# mset CS))\<close> and
+    is_\<L>\<^sub>a\<^sub>l\<^sub>l: \<open>is_\<L>\<^sub>a\<^sub>l\<^sub>l (all_lits_of_mm (mset `# mset CS))\<close> and
     lits_upd_confl: \<open>get_conflict_wl S \<noteq> None \<longrightarrow> literals_to_update_wl S = {#}\<close>
   shows
     \<open>init_dt_wl CS S \<le> SPEC(\<lambda>T.
-      is_N\<^sub>1 (all_lits_of_mm (mset `# mset CS +
+      is_\<L>\<^sub>a\<^sub>l\<^sub>l (all_lits_of_mm (mset `# mset CS +
           cdcl\<^sub>W_restart_mset.clauses (state\<^sub>W_of (twl_st_of None (st_l_of_wl None S))))) \<and>
        twl_struct_invs (twl_st_of_wl None T) \<and> twl_stgy_invs (twl_st_of_wl None T) \<and>
        additional_WS_invs (st_l_of_wl None T) \<and>
@@ -1074,8 +1074,8 @@ lemma init_dt_init_dt_l_full:
       (get_conflict_wl T \<noteq> None \<longrightarrow> literals_to_update_wl T = {#}))\<close>
 proof -
   define T where \<open>T = st_l_of_wl None S\<close>
-  have CS_N\<^sub>1: \<open>\<forall>C\<in>set CS. literals_are_in_N\<^sub>0 (mset C)\<close>
-    using is_N\<^sub>1 all_lits_of_mm_in_all_lits_of_m_in_iff unfolding is_N\<^sub>1_def literals_are_in_N\<^sub>0_def
+  have CS_\<L>\<^sub>a\<^sub>l\<^sub>l: \<open>\<forall>C\<in>set CS. literals_are_in_\<A>\<^sub>i\<^sub>n (mset C)\<close>
+    using is_\<L>\<^sub>a\<^sub>l\<^sub>l all_lits_of_mm_in_all_lits_of_m_in_iff unfolding is_\<L>\<^sub>a\<^sub>l\<^sub>l_def literals_are_in_\<A>\<^sub>i\<^sub>n_def
     by blast
   have w_q: \<open>clauses_to_update_l T = {#}\<close>
     by (cases S) (simp add: T_def)
@@ -1112,17 +1112,17 @@ proof -
     done
   have Un_eq_iff_subset: \<open>A \<union> B = A \<longleftrightarrow> B \<subseteq> A\<close> for A B
     by blast
-  have [simp]: \<open>twl_array_code_ops.is_N\<^sub>1 N\<^sub>0 (A + all_lits_of_mm B) \<longleftrightarrow>
-       set_mset (all_lits_of_mm B) \<subseteq> set_mset N\<^sub>1\<close>
-    if \<open>twl_array_code_ops.is_N\<^sub>1 N\<^sub>0 A\<close> for A B
-    using that by (simp add: twl_array_code_ops.is_N\<^sub>1_def twl_array_code_ops.literals_are_in_N\<^sub>0_def
+  have [simp]: \<open>twl_array_code_ops.is_\<L>\<^sub>a\<^sub>l\<^sub>l \<A>\<^sub>i\<^sub>n (A + all_lits_of_mm B) \<longleftrightarrow>
+       set_mset (all_lits_of_mm B) \<subseteq> set_mset \<L>\<^sub>a\<^sub>l\<^sub>l\<close>
+    if \<open>twl_array_code_ops.is_\<L>\<^sub>a\<^sub>l\<^sub>l \<A>\<^sub>i\<^sub>n A\<close> for A B
+    using that by (simp add: twl_array_code_ops.is_\<L>\<^sub>a\<^sub>l\<^sub>l_def twl_array_code_ops.literals_are_in_\<A>\<^sub>i\<^sub>n_def
         Un_eq_iff_subset)
-  have CS_N\<^sub>1': \<open>set_mset (all_lits_of_mm (mset `# mset CS)) \<subseteq> set_mset N\<^sub>1\<close>
-    using is_N\<^sub>1 unfolding twl_array_code_ops.is_N\<^sub>1_def by (clarsimp simp: HH_def all_lits_of_mm_union)
+  have CS_\<L>\<^sub>a\<^sub>l\<^sub>l': \<open>set_mset (all_lits_of_mm (mset `# mset CS)) \<subseteq> set_mset \<L>\<^sub>a\<^sub>l\<^sub>l\<close>
+    using is_\<L>\<^sub>a\<^sub>l\<^sub>l unfolding twl_array_code_ops.is_\<L>\<^sub>a\<^sub>l\<^sub>l_def by (clarsimp simp: HH_def all_lits_of_mm_union)
   have \<open>set_mset (all_lits_of_mm (cdcl\<^sub>W_restart_mset.clauses
       (state\<^sub>W_of (twl_st_of None (st_l_of_wl None S))))) \<subseteq>
-   set_mset N\<^sub>1\<close>
-    using S_N\<^sub>1 unfolding twl_array_code_ops.is_N\<^sub>1_def
+   set_mset \<L>\<^sub>a\<^sub>l\<^sub>l\<close>
+    using S_\<L>\<^sub>a\<^sub>l\<^sub>l unfolding twl_array_code_ops.is_\<L>\<^sub>a\<^sub>l\<^sub>l_def
     by (cases S)(clarsimp simp: mset_take_mset_drop_mset' clauses_def HH_def cl_T_S)
   have [simp]: \<open>mset `# mset (take ag (tl af)) + ai + (mset `# mset (drop (Suc ag) af)) =
      mset `# mset (tl af) + ai\<close> for ag af aj ai
@@ -1130,16 +1130,16 @@ proof -
       (auto simp: drop_Suc)
   show ?thesis
     apply (rule order.trans)
-     apply (rule conc_trans[OF init_dt_wl_init_dt_l i, of S, unfolded N\<^sub>1_def[symmetric]])
-    subgoal using clss watch S_N\<^sub>1 no_learned trail_in_NP prop_NP lits_upd_confl
+     apply (rule conc_trans[OF init_dt_wl_init_dt_l i, of S, unfolded \<L>\<^sub>a\<^sub>l\<^sub>l_def[symmetric]])
+    subgoal using clss watch S_\<L>\<^sub>a\<^sub>l\<^sub>l no_learned trail_in_NP prop_NP lits_upd_confl
       by (auto simp: HH_def T_def clauses_def mset_take_mset_drop_mset' get_unit_learned_def
-            get_unit_init_clss_def N\<^sub>1_def
+            get_unit_init_clss_def \<L>\<^sub>a\<^sub>l\<^sub>l_def
           simp del: correct_watching_init.simps literal_of_nat.simps)
-    subgoal using CS_N\<^sub>1 by auto
+    subgoal using CS_\<L>\<^sub>a\<^sub>l\<^sub>l by auto
     subgoal using dist .
-    subgoal using is_N\<^sub>1 CS_N\<^sub>1' S_N\<^sub>1 unfolding conc_fun_RES
+    subgoal using is_\<L>\<^sub>a\<^sub>l\<^sub>l CS_\<L>\<^sub>a\<^sub>l\<^sub>l' S_\<L>\<^sub>a\<^sub>l\<^sub>l unfolding conc_fun_RES
       by (clarsimp simp: HH_def all_lits_of_mm_union mset_take_mset_drop_mset'
-          clauses_def get_unit_learned_def get_unit_init_clss_def N\<^sub>1_def
+          clauses_def get_unit_learned_def get_unit_init_clss_def \<L>\<^sub>a\<^sub>l\<^sub>l_def
           simp del: literal_of_nat.simps)
     done
 qed
@@ -1151,10 +1151,10 @@ lemma init_dt_init_dt_l:
     dist: \<open>\<forall>C \<in> set CS. distinct C\<close> and
     length: \<open>\<forall>C \<in> set CS. length C \<ge> 1\<close> and
     upper: \<open>\<forall>C\<in>set CS. \<forall>L\<in>set C. nat_of_lit L < upperN\<close> and
-    is_N\<^sub>1: \<open>is_N\<^sub>1 (all_lits_of_mm (mset `# mset CS))\<close>
+    is_\<L>\<^sub>a\<^sub>l\<^sub>l: \<open>is_\<L>\<^sub>a\<^sub>l\<^sub>l (all_lits_of_mm (mset `# mset CS))\<close>
   shows
     \<open>init_dt_wl CS S \<le> SPEC(\<lambda>S.
-       is_N\<^sub>1 (all_lits_of_mm (mset `# mset CS)) \<and>
+       is_\<L>\<^sub>a\<^sub>l\<^sub>l (all_lits_of_mm (mset `# mset CS)) \<and>
        twl_struct_invs (twl_st_of_wl None S) \<and> twl_stgy_invs (twl_st_of_wl None S) \<and>
        correct_watching S \<and>
        additional_WS_invs (st_l_of_wl None S) \<and>
@@ -1179,8 +1179,8 @@ proof -
     stgy_invs: \<open>twl_stgy_invs (twl_st_of_wl None S)\<close> and
     watch: \<open>correct_watching_init S\<close> and
     clss: \<open>get_clauses_wl S \<noteq> []\<close> and
-    S_N\<^sub>1: \<open>set_mset (all_lits_of_mm (cdcl\<^sub>W_restart_mset.clauses
-      (state\<^sub>W_of (twl_st_of None (st_l_of_wl None S))))) \<subseteq> set_mset N\<^sub>1\<close> and
+    S_\<L>\<^sub>a\<^sub>l\<^sub>l: \<open>set_mset (all_lits_of_mm (cdcl\<^sub>W_restart_mset.clauses
+      (state\<^sub>W_of (twl_st_of None (st_l_of_wl None S))))) \<subseteq> set_mset \<L>\<^sub>a\<^sub>l\<^sub>l\<close> and
     no_learned: \<open>(\<lambda>(M, N, U, D, NP, UP, Q, W). UP) S = {#}\<close> and
     learned_nil: \<open>get_unit_learned S = {#}\<close> and
     confl_nil: \<open>get_conflict_wl S = None\<close> and
@@ -1201,30 +1201,30 @@ proof -
      mset `# mset (tl af) + ai\<close> for ag af aj ai
     by (subst (2) append_take_drop_id[symmetric, of \<open>tl af\<close> ag], subst mset_append)
       (auto simp: drop_Suc)
-  have \<open>set_mset N\<^sub>1 \<subseteq> set_mset (all_lits_of_m N\<^sub>1)\<close>
-    by (fastforce simp: all_lits_of_m_def N\<^sub>1_def image_image uminus_lit_swap)
-  then have [simp]: \<open>set_mset (all_lits_of_m N\<^sub>1) = set_mset N\<^sub>1\<close>
-    by (fastforce simp: all_lits_of_m_def N\<^sub>1_def image_image uminus_lit_swap
+  have \<open>set_mset \<L>\<^sub>a\<^sub>l\<^sub>l \<subseteq> set_mset (all_lits_of_m \<L>\<^sub>a\<^sub>l\<^sub>l)\<close>
+    by (fastforce simp: all_lits_of_m_def \<L>\<^sub>a\<^sub>l\<^sub>l_def image_image uminus_lit_swap)
+  then have [simp]: \<open>set_mset (all_lits_of_m \<L>\<^sub>a\<^sub>l\<^sub>l) = set_mset \<L>\<^sub>a\<^sub>l\<^sub>l\<close>
+    by (fastforce simp: all_lits_of_m_def \<L>\<^sub>a\<^sub>l\<^sub>l_def image_image uminus_lit_swap
         simp del: literal_of_nat.simps)
-  have [simp]: \<open>all_lits_of_atms_m N\<^sub>0 = N\<^sub>1\<close>
-    by (simp add: N\<^sub>1_def all_lits_of_atms_m_def)
+  have [simp]: \<open>all_lits_of_atms_m \<A>\<^sub>i\<^sub>n = \<L>\<^sub>a\<^sub>l\<^sub>l\<close>
+    by (simp add: \<L>\<^sub>a\<^sub>l\<^sub>l_def all_lits_of_atms_m_def)
   show ?thesis
     apply (rule order.trans)
      apply (rule HH)
-    using upper is_N\<^sub>1
-    by (clarsimp_all simp: correct_watching.simps twl_array_code_ops.is_N\<^sub>1_def clauses_def
+    using upper is_\<L>\<^sub>a\<^sub>l\<^sub>l
+    by (clarsimp_all simp: correct_watching.simps twl_array_code_ops.is_\<L>\<^sub>a\<^sub>l\<^sub>l_def clauses_def
         mset_take_mset_drop_mset' get_unit_learned_def confl_nil trail_in_NP prop_NP)
 qed
 
 definition (in twl_array_code_ops) init_state :: \<open>nat clauses \<Rightarrow> nat cdcl\<^sub>W_restart_mset\<close> where
   \<open>init_state N = (
-    let _ = N\<^sub>0 in
+    let _ = \<A>\<^sub>i\<^sub>n in
     ([]:: (nat, nat clause) ann_lits), (N :: nat clauses), ({#}::nat clauses),
       (None :: nat clause option))\<close>
 
 text \<open>We add a spurious depency to the parameter of the locale:\<close>
 definition (in twl_array_code_ops) empty_watched :: \<open>nat literal \<Rightarrow> nat list\<close> where
-  \<open>empty_watched = (let _ = N\<^sub>0 in (\<lambda>_. []))\<close>
+  \<open>empty_watched = (let _ = \<A>\<^sub>i\<^sub>n in (\<lambda>_. []))\<close>
 
 lemma (in twl_array_code_ops) empty_watched_alt_def:
   \<open>empty_watched = (\<lambda>_. [])\<close>
@@ -1267,11 +1267,11 @@ definition SAT :: \<open>nat clauses \<Rightarrow> nat cdcl\<^sub>W_restart_mset
 definition (in -) SAT_wl :: \<open>nat clauses_l \<Rightarrow> nat twl_st_wl nres\<close> where
   \<open>SAT_wl CS = do{
     let n = length CS;
-    let N\<^sub>0' = extract_atms_clss CS [];
-    let S = twl_array_code_ops.init_state_wl (mset N\<^sub>0');
-    T \<leftarrow> twl_array_code.init_dt_wl (mset N\<^sub>0') CS S;
+    let \<A>\<^sub>i\<^sub>n' = extract_atms_clss CS [];
+    let S = twl_array_code_ops.init_state_wl (mset \<A>\<^sub>i\<^sub>n');
+    T \<leftarrow> twl_array_code.init_dt_wl (mset \<A>\<^sub>i\<^sub>n') CS S;
     if get_conflict_wl T = None
-    then twl_array_code.cdcl_twl_stgy_prog_wl_D (mset N\<^sub>0') (finalise_init T)
+    then twl_array_code.cdcl_twl_stgy_prog_wl_D (mset \<A>\<^sub>i\<^sub>n') (finalise_init T)
     else RETURN T
   }\<close>
 
@@ -1444,19 +1444,19 @@ proof -
   have [simp]: \<open>twl_array_code_ops.abs_l_vmtf_remove_inv N [] ((nat_of_uint32 ` set N', {}), {})\<close>
     if \<open>(N', y) \<in> \<langle>uint32_nat_rel\<rangle>list_rel\<close> and \<open>(y, N) \<in> list_mset_rel\<close> for N N' y
     using that unfolding twl_array_code_ops.abs_l_vmtf_remove_inv_def
-    by (auto simp: twl_array_code_ops.N\<^sub>1_def atms_of_def image_image image_Un list_rel_def
+    by (auto simp: twl_array_code_ops.\<L>\<^sub>a\<^sub>l\<^sub>l_def atms_of_def image_image image_Un list_rel_def
       uint32_nat_rel_def br_def list_mset_rel_def list_all2_op_eq_map_right_iff')
-  have in_N_in_N1: \<open>L \<in> set N' \<Longrightarrow>  nat_of_uint32 L \<in> atms_of (twl_array_code_ops.N\<^sub>1 N)\<close>
+  have in_N_in_N1: \<open>L \<in> set N' \<Longrightarrow>  nat_of_uint32 L \<in> atms_of (twl_array_code_ops.\<L>\<^sub>a\<^sub>l\<^sub>l N)\<close>
     if \<open>(N', y) \<in> \<langle>uint32_nat_rel\<rangle>list_rel\<close> and \<open>(y, N) \<in> list_mset_rel\<close> for L N N' y
-    using that by (auto simp: twl_array_code_ops.N\<^sub>1_def atms_of_def image_image image_Un list_rel_def
+    using that by (auto simp: twl_array_code_ops.\<L>\<^sub>a\<^sub>l\<^sub>l_def atms_of_def image_image image_Un list_rel_def
       uint32_nat_rel_def br_def list_mset_rel_def list_all2_op_eq_map_right_iff')
 
-  have length_ba: \<open>\<forall>L\<in># N. L < length ba \<Longrightarrow> L \<in> atms_of (twl_array_code_ops.N\<^sub>1 N) \<Longrightarrow>
+  have length_ba: \<open>\<forall>L\<in># N. L < length ba \<Longrightarrow> L \<in> atms_of (twl_array_code_ops.\<L>\<^sub>a\<^sub>l\<^sub>l N) \<Longrightarrow>
      L < length ba\<close>
     if \<open>(N', y) \<in> \<langle>uint32_nat_rel\<rangle>list_rel\<close> and \<open>(y, N) \<in> list_mset_rel\<close>
     for L ba N N' y
     using that
-    by (auto simp: twl_array_code_ops.N\<^sub>1_def nat_shiftr_div2 nat_of_uint32_shiftr
+    by (auto simp: twl_array_code_ops.\<L>\<^sub>a\<^sub>l\<^sub>l_def nat_shiftr_div2 nat_of_uint32_shiftr
       atms_of_def image_image image_Un split: if_splits)
   show ?thesis
     apply (intro frefI nres_relI)
@@ -1513,15 +1513,15 @@ definition extract_model_of_state where
 definition IsaSAT :: \<open>nat clauses_l \<Rightarrow> nat literal list option nres\<close> where
   \<open>IsaSAT CS = do{
     let n = length CS;
-    let N\<^sub>0' = mset (extract_atms_clss CS []);
-    ASSERT(twl_array_code N\<^sub>0');
-    ASSERT(distinct_mset N\<^sub>0');
-    let S = twl_array_code_ops.init_state_wl N\<^sub>0';
-    T \<leftarrow> twl_array_code.init_dt_wl N\<^sub>0' CS S;
+    let \<A>\<^sub>i\<^sub>n' = mset (extract_atms_clss CS []);
+    ASSERT(twl_array_code \<A>\<^sub>i\<^sub>n');
+    ASSERT(distinct_mset \<A>\<^sub>i\<^sub>n');
+    let S = twl_array_code_ops.init_state_wl \<A>\<^sub>i\<^sub>n';
+    T \<leftarrow> twl_array_code.init_dt_wl \<A>\<^sub>i\<^sub>n' CS S;
     if get_conflict_wl_is_None_no_clvls T
     then do {
        let T = finalise_init T;
-       U \<leftarrow> twl_array_code.cdcl_twl_stgy_prog_wl_D N\<^sub>0' T;
+       U \<leftarrow> twl_array_code.cdcl_twl_stgy_prog_wl_D \<A>\<^sub>i\<^sub>n' T;
        RETURN (if get_conflict_wl U = None then Some (extract_model_of_state U) else None)}
     else RETURN None
   }\<close>
@@ -1550,7 +1550,7 @@ lemma shiftr1_fref[sepref_fr_rules]: \<open>(return o shiftr1, RETURN o shiftr1)
 
 
 definition init_trail_D :: \<open>uint32 list \<Rightarrow> nat \<Rightarrow> trail_int nres\<close> where
-  \<open>init_trail_D N\<^sub>0 n = do {
+  \<open>init_trail_D \<A>\<^sub>i\<^sub>n n = do {
      let M = replicate n None;
      let M' = replicate n zero_uint32_nat;
      RETURN (([], M, M', zero_uint32_nat))
@@ -1576,16 +1576,16 @@ declare init_trail_D_code.refine[sepref_fr_rules]
 
 definition init_state_wl_D' :: \<open>uint32 list \<Rightarrow>  (trail_int \<times> _ list list \<times>
      nat \<times> _) nres\<close> where
-  \<open>init_state_wl_D' N\<^sub>0 = do {
-     let n = Suc (nat_of_uint32 (fold max N\<^sub>0 0));
+  \<open>init_state_wl_D' \<A>\<^sub>i\<^sub>n = do {
+     let n = Suc (nat_of_uint32 (fold max \<A>\<^sub>i\<^sub>n 0));
      let m = 2 * n;
-     M \<leftarrow> init_trail_D N\<^sub>0 n;
+     M \<leftarrow> init_trail_D \<A>\<^sub>i\<^sub>n n;
      let e = [];
      let N = init_rll n;
      let N = N @ [e];
      let D = (True, zero_uint32_nat, replicate n None);
      let WS = init_lrl m;
-     vm \<leftarrow> initialise_VMTF N\<^sub>0 n;
+     vm \<leftarrow> initialise_VMTF \<A>\<^sub>i\<^sub>n n;
      let \<phi> = replicate n False;
 
      RETURN (M, N, 0, D, [], WS, vm, \<phi>, zero_uint32_nat)
@@ -1622,15 +1622,15 @@ sepref_definition init_state_wl_D'_code
   by sepref
 
 lemma init_trail_D_ref:
-  \<open>(uncurry init_trail_D, uncurry (RETURN oo (\<lambda> _ _. []))) \<in> [\<lambda>(N, n). mset N = N\<^sub>0 \<and>
+  \<open>(uncurry init_trail_D, uncurry (RETURN oo (\<lambda> _ _. []))) \<in> [\<lambda>(N, n). mset N = \<A>\<^sub>i\<^sub>n \<and>
     distinct N \<and> (\<forall>L\<in>set N. L< n)]\<^sub>f
     \<langle>uint32_nat_rel\<rangle>list_rel \<times>\<^sub>r nat_rel \<rightarrow>
-   \<langle>twl_array_code_ops.trailt_ref N\<^sub>0\<rangle> nres_rel\<close>
+   \<langle>twl_array_code_ops.trailt_ref \<A>\<^sub>i\<^sub>n\<rangle> nres_rel\<close>
 proof -
   have K: \<open>(\<forall>L\<in>set N. nat_of_uint32 L < n) \<longleftrightarrow>
-     (\<forall>L \<in># (twl_array_code_ops.N\<^sub>1 (nat_of_uint32 `# mset N)). atm_of L < n)\<close> for N n
+     (\<forall>L \<in># (twl_array_code_ops.\<L>\<^sub>a\<^sub>l\<^sub>l (nat_of_uint32 `# mset N)). atm_of L < n)\<close> for N n
      (*TODO proof*)
-    apply (auto simp: nat_shiftr_div2 nat_of_uint32_shiftr twl_array_code_ops.N\<^sub>1_def)
+    apply (auto simp: nat_shiftr_div2 nat_of_uint32_shiftr twl_array_code_ops.\<L>\<^sub>a\<^sub>l\<^sub>l_def)
     by (metis (full_types) UnCI image_eqI literal.sel(1))
 
   show ?thesis
@@ -1639,7 +1639,7 @@ proof -
     unfolding uncurry_def Let_def comp_def
     apply clarify
     by (auto 5 5 simp: zero_uint32_def twl_array_code_ops.trailt_ref_def shiftr1_def
-        nat_shiftr_div2 nat_of_uint32_shiftr twl_array_code_ops.in_N\<^sub>1_atm_of_in_atms_of_iff
+        nat_shiftr_div2 nat_of_uint32_shiftr twl_array_code_ops.in_\<L>\<^sub>a\<^sub>l\<^sub>l_atm_of_in_atms_of_iff
         valued_atm_on_trail_def twl_array_code_ops.trailt_ref_def K atms_of_def
         twl_array_code_ops.phase_saving_def list_rel_mset_rel_def
         list_rel_def uint32_nat_rel_def br_def list_all2_op_eq_map_right_iff'
@@ -1648,23 +1648,23 @@ qed
 
 lemma init_state_wl_D':
   \<open>(init_state_wl_D', twl_array_code_ops.init_state_wl_int) \<in>
-    [\<lambda>N. N = N\<^sub>0 \<and> distinct_mset N\<^sub>0]\<^sub>f \<langle>uint32_nat_rel\<rangle>list_rel_mset_rel  \<rightarrow>
-      \<langle>twl_array_code_ops.trailt_ref N\<^sub>0 \<times>\<^sub>r \<langle>\<langle>Id\<rangle>list_rel\<rangle>list_rel \<times>\<^sub>r
-         nat_rel \<times>\<^sub>r twl_array_code_ops.option_conflict_rel N\<^sub>0 \<times>\<^sub>r list_mset_rel \<times>\<^sub>r \<langle>\<langle>Id\<rangle>list_rel\<rangle>list_rel \<times>\<^sub>r
+    [\<lambda>N. N = \<A>\<^sub>i\<^sub>n \<and> distinct_mset \<A>\<^sub>i\<^sub>n]\<^sub>f \<langle>uint32_nat_rel\<rangle>list_rel_mset_rel  \<rightarrow>
+      \<langle>twl_array_code_ops.trailt_ref \<A>\<^sub>i\<^sub>n \<times>\<^sub>r \<langle>\<langle>Id\<rangle>list_rel\<rangle>list_rel \<times>\<^sub>r
+         nat_rel \<times>\<^sub>r twl_array_code_ops.option_conflict_rel \<A>\<^sub>i\<^sub>n \<times>\<^sub>r list_mset_rel \<times>\<^sub>r \<langle>\<langle>Id\<rangle>list_rel\<rangle>list_rel \<times>\<^sub>r
            Id \<times>\<^sub>r \<langle>bool_rel\<rangle>list_rel\<times>\<^sub>r Id\<rangle>nres_rel\<close>
 proof -
-  have init_state_wl_int_alt_def: \<open>twl_array_code_ops.init_state_wl_int N\<^sub>0 = do {
+  have init_state_wl_int_alt_def: \<open>twl_array_code_ops.init_state_wl_int \<A>\<^sub>i\<^sub>n = do {
     let M = [];
     let N = [[]];
     let D = None;
-    W \<leftarrow> SPEC (\<lambda>W. (W, twl_array_code_ops.empty_watched N\<^sub>0 ) \<in> \<langle>Id\<rangle>map_fun_rel (twl_array_code_ops.D\<^sub>0 N\<^sub>0));
-    vm \<leftarrow> RES (twl_array_code_ops.vmtf_imp N\<^sub>0 []);
-    \<phi> \<leftarrow> SPEC (twl_array_code_ops.phase_saving N\<^sub>0);
-    RETURN (M, N, 0, D, {#}, W, vm, \<phi>, zero_uint32_nat)}\<close> for N\<^sub>0
+    W \<leftarrow> SPEC (\<lambda>W. (W, twl_array_code_ops.empty_watched \<A>\<^sub>i\<^sub>n ) \<in> \<langle>Id\<rangle>map_fun_rel (twl_array_code_ops.D\<^sub>0 \<A>\<^sub>i\<^sub>n));
+    vm \<leftarrow> RES (twl_array_code_ops.vmtf_imp \<A>\<^sub>i\<^sub>n []);
+    \<phi> \<leftarrow> SPEC (twl_array_code_ops.phase_saving \<A>\<^sub>i\<^sub>n);
+    RETURN (M, N, 0, D, {#}, W, vm, \<phi>, zero_uint32_nat)}\<close> for \<A>\<^sub>i\<^sub>n
     unfolding twl_array_code_ops.init_state_wl_int_def Let_def by auto
 
-  have tr: \<open>distinct_mset N\<^sub>0 \<and> (\<forall>L\<in>#N\<^sub>0. L < b) \<Longrightarrow> (N\<^sub>0', N\<^sub>0) \<in> \<langle>uint32_nat_rel\<rangle>list_rel_mset_rel \<Longrightarrow>
-      init_trail_D N\<^sub>0' b \<le> \<Down> (twl_array_code_ops.trailt_ref N\<^sub>0) (RETURN [])\<close> for b N\<^sub>0 N\<^sub>0' x
+  have tr: \<open>distinct_mset \<A>\<^sub>i\<^sub>n \<and> (\<forall>L\<in>#\<A>\<^sub>i\<^sub>n. L < b) \<Longrightarrow> (\<A>\<^sub>i\<^sub>n', \<A>\<^sub>i\<^sub>n) \<in> \<langle>uint32_nat_rel\<rangle>list_rel_mset_rel \<Longrightarrow>
+      init_trail_D \<A>\<^sub>i\<^sub>n' b \<le> \<Down> (twl_array_code_ops.trailt_ref \<A>\<^sub>i\<^sub>n) (RETURN [])\<close> for b \<A>\<^sub>i\<^sub>n \<A>\<^sub>i\<^sub>n' x
     by (rule init_trail_D_ref[unfolded fref_def nres_rel_def, simplified, rule_format])
        (auto simp: list_rel_mset_rel_def list_mset_rel_def br_def)
   have [simp]: \<open>comp_fun_idem (max :: 'a::linorder \<Rightarrow> _)\<close>
@@ -1672,18 +1672,18 @@ proof -
     by (auto simp: max_def[abs_def] intro!: ext)
   have [simp]: \<open>fold max x a = Max (insert a (set x))\<close> for x and a :: \<open>'a :: linorder\<close>
     by (auto simp: Max.eq_fold comp_fun_idem.fold_set_fold)
-  have in_N0[dest]: \<open>L \<in> set N\<^sub>0 \<Longrightarrow> nat_of_uint32 L  < Suc (nat_of_uint32 (Max (insert 0 (set N\<^sub>0))))\<close>
-    for L N\<^sub>0
-    using Max_ge[of \<open>insert 0 (set N\<^sub>0)\<close> L]
+  have in_N0[dest]: \<open>L \<in> set \<A>\<^sub>i\<^sub>n \<Longrightarrow> nat_of_uint32 L  < Suc (nat_of_uint32 (Max (insert 0 (set \<A>\<^sub>i\<^sub>n))))\<close>
+    for L \<A>\<^sub>i\<^sub>n
+    using Max_ge[of \<open>insert 0 (set \<A>\<^sub>i\<^sub>n)\<close> L]
     apply (auto simp del: Max_ge simp: nat_shiftr_div2 nat_of_uint32_shiftr)
     using div_le_mono le_imp_less_Suc nat_of_uint32_le_iff by blast
   define P where \<open>P x = {(a, b). b = [] \<and> (a, b) \<in> twl_array_code_ops.trailt_ref x}\<close> for x
   have P: \<open>(c, []) \<in> P x \<longleftrightarrow> (c, []) \<in> twl_array_code_ops.trailt_ref x\<close> for c x
     unfolding P_def by auto
-  have init: \<open>init_trail_D N\<^sub>0' (Suc (nat_of_uint32 (fold max N\<^sub>0' 0))) \<le>
-     SPEC (\<lambda>c. (c, []) \<in> P N\<^sub>0)\<close>
-    if \<open>distinct_mset N\<^sub>0\<close> and x: \<open>(N\<^sub>0', N\<^sub>0) \<in> \<langle>uint32_nat_rel\<rangle>list_rel_mset_rel\<close>
-    for N\<^sub>0 N\<^sub>0'
+  have init: \<open>init_trail_D \<A>\<^sub>i\<^sub>n' (Suc (nat_of_uint32 (fold max \<A>\<^sub>i\<^sub>n' 0))) \<le>
+     SPEC (\<lambda>c. (c, []) \<in> P \<A>\<^sub>i\<^sub>n)\<close>
+    if \<open>distinct_mset \<A>\<^sub>i\<^sub>n\<close> and x: \<open>(\<A>\<^sub>i\<^sub>n', \<A>\<^sub>i\<^sub>n) \<in> \<langle>uint32_nat_rel\<rangle>list_rel_mset_rel\<close>
+    for \<A>\<^sub>i\<^sub>n \<A>\<^sub>i\<^sub>n'
     unfolding x P
     by (rule tr[unfolded conc_fun_RETURN])
        (use that in \<open>auto simp: shiftr1_def nat_shiftr_div2 nat_of_uint32_shiftr list_rel_mset_rel_def
@@ -1693,12 +1693,12 @@ proof -
     by (auto simp: list_mset_rel_def br_def)
   have H:
    \<open>(replicate (Suc (Suc (2 * nat_of_uint32 (Max (insert 0 (set x)))))) [],
-       twl_array_code_ops.empty_watched N\<^sub>0)
-    \<in> \<langle>Id\<rangle>map_fun_rel ((\<lambda>L. (nat_of_lit L, L)) ` set_mset (twl_array_code_ops.N\<^sub>1 N\<^sub>0))\<close>
-    if \<open>(x, N\<^sub>0) \<in> \<langle>uint32_nat_rel\<rangle>list_rel_mset_rel\<close>
-    for N\<^sub>0 x
+       twl_array_code_ops.empty_watched \<A>\<^sub>i\<^sub>n)
+    \<in> \<langle>Id\<rangle>map_fun_rel ((\<lambda>L. (nat_of_lit L, L)) ` set_mset (twl_array_code_ops.\<L>\<^sub>a\<^sub>l\<^sub>l \<A>\<^sub>i\<^sub>n))\<close>
+    if \<open>(x, \<A>\<^sub>i\<^sub>n) \<in> \<langle>uint32_nat_rel\<rangle>list_rel_mset_rel\<close>
+    for \<A>\<^sub>i\<^sub>n x
     using that unfolding map_fun_rel_def
-    by (auto simp: twl_array_code_ops.empty_watched_def twl_array_code_ops.N\<^sub>1_def
+    by (auto simp: twl_array_code_ops.empty_watched_def twl_array_code_ops.\<L>\<^sub>a\<^sub>l\<^sub>l_def
       list_rel_mset_rel_def list_rel_mset_rel_def
       list_rel_def uint32_nat_rel_def br_def list_all2_op_eq_map_right_iff' list_mset_rel_def
      intro!: nth_replicate dest!: in_N0
@@ -1716,10 +1716,10 @@ proof -
     if \<open>(x, y) \<in> \<langle>uint32_nat_rel\<rangle>list_rel_mset_rel\<close> and \<open>(M, []) \<in> P y\<close> and \<open>distinct_mset y\<close> for x y M
     using that
     by (auto simp: P_def intro!: initialise_VMTF in_N0)
-  have [simp]: \<open>(x, N\<^sub>0) \<in> \<langle>uint32_nat_rel\<rangle>list_rel_mset_rel \<Longrightarrow>
-         L \<in> atms_of (twl_array_code_ops.N\<^sub>1 N\<^sub>0) \<Longrightarrow> L < Suc (nat_of_uint32 (Max (insert 0 (set x))))\<close>
-    for x L N\<^sub>0
-    unfolding twl_array_code_ops.atms_of_N\<^sub>1_N\<^sub>0
+  have [simp]: \<open>(x, \<A>\<^sub>i\<^sub>n) \<in> \<langle>uint32_nat_rel\<rangle>list_rel_mset_rel \<Longrightarrow>
+         L \<in> atms_of (twl_array_code_ops.\<L>\<^sub>a\<^sub>l\<^sub>l \<A>\<^sub>i\<^sub>n) \<Longrightarrow> L < Suc (nat_of_uint32 (Max (insert 0 (set x))))\<close>
+    for x L \<A>\<^sub>i\<^sub>n
+    unfolding twl_array_code_ops.atms_of_\<L>\<^sub>a\<^sub>l\<^sub>l_\<A>\<^sub>i\<^sub>n
     by (auto simp: list_rel_mset_rel_def br_def list_rel_def uint32_nat_rel_def
         list_all2_op_eq_map_right_iff' list_mset_rel_def)
 
@@ -1747,26 +1747,26 @@ qed
 
 lemma init_state_wl_int_hnr:
   \<open>(init_state_wl_D'_code, twl_array_code_ops.init_state_wl_int)
-    \<in> [\<lambda>x. x = N\<^sub>0 \<and> distinct_mset N\<^sub>0]\<^sub>a
+    \<in> [\<lambda>x. x = \<A>\<^sub>i\<^sub>n \<and> distinct_mset \<A>\<^sub>i\<^sub>n]\<^sub>a
       (hr_comp (list_assn uint32_assn) (\<langle>uint32_nat_rel\<rangle>list_rel_mset_rel))\<^sup>k \<rightarrow>
-      twl_array_code_ops.twl_st_int_assn N\<^sub>0\<close>
+      twl_array_code_ops.twl_st_int_assn \<A>\<^sub>i\<^sub>n\<close>
     (is \<open>?c \<in> [?pre]\<^sub>a ?im \<rightarrow> ?f\<close>)
 proof -
   have H: \<open>?c
-  \<in> [\<lambda>x. x = N\<^sub>0 \<and>
+  \<in> [\<lambda>x. x = \<A>\<^sub>i\<^sub>n \<and>
           distinct_mset
-           N\<^sub>0]\<^sub>a (hr_comp (list_assn uint32_assn)
+           \<A>\<^sub>i\<^sub>n]\<^sub>a (hr_comp (list_assn uint32_assn)
                     (\<langle>uint32_nat_rel\<rangle>list_rel_mset_rel))\<^sup>k \<rightarrow>
-      hr_comp trailt_conc (twl_array_code_ops.trailt_ref N\<^sub>0) *assn
+      hr_comp trailt_conc (twl_array_code_ops.trailt_ref \<A>\<^sub>i\<^sub>n) *assn
       hr_comp clauses_ll_assn (\<langle>\<langle>nat_lit_lit_rel\<rangle>list_rel\<rangle>list_rel) *assn
       nat_assn *assn
-      hr_comp conflict_option_rel_assn (twl_array_code_ops.option_conflict_rel N\<^sub>0) *assn
+      hr_comp conflict_option_rel_assn (twl_array_code_ops.option_conflict_rel \<A>\<^sub>i\<^sub>n) *assn
       hr_comp (list_assn unat_lit_assn) list_mset_rel *assn
       hr_comp (arrayO_assn (arl_assn nat_assn)) (\<langle>\<langle>nat_rel\<rangle>list_rel\<rangle>list_rel) *assn
       vmtf_remove_conc *assn hr_comp phase_saver_conc (\<langle>bool_rel\<rangle>list_rel) *assn
       uint32_nat_assn\<close>
     (is \<open>_ \<in> [?pre']\<^sub>a ?im' \<rightarrow> ?f'\<close>)
-    using  init_state_wl_D'_code.refine[FCOMP init_state_wl_D', of N\<^sub>0] .
+    using  init_state_wl_D'_code.refine[FCOMP init_state_wl_D', of \<A>\<^sub>i\<^sub>n] .
   have pre: \<open>?pre x \<Longrightarrow> ?pre' x\<close> for x
     unfolding comp_PRE_def by fast
   have im: \<open>?im' = ?im\<close>
@@ -1785,30 +1785,30 @@ qed
 
 lemma init_state_wl_int_init_state_wl:
   \<open>(twl_array_code_ops.init_state_wl_int, RETURN o twl_array_code_ops.init_state_wl)
-  \<in> [\<lambda>N. N = N\<^sub>0]\<^sub>f Id \<rightarrow> \<langle>twl_array_code_ops.twl_st_ref_no_clvls
-                    N\<^sub>0\<rangle>nres_rel\<close>
+  \<in> [\<lambda>N. N = \<A>\<^sub>i\<^sub>n]\<^sub>f Id \<rightarrow> \<langle>twl_array_code_ops.twl_st_ref_no_clvls
+                    \<A>\<^sub>i\<^sub>n\<rangle>nres_rel\<close>
   using twl_array_code_ops.init_state_wl_int_init_state_wl
   unfolding fref_def nres_rel_def
   by auto
 
 lemma init_state_wl_D'_code_ref[sepref_fr_rules]:
   \<open>(init_state_wl_D'_code, RETURN o twl_array_code_ops.init_state_wl) \<in>
-    [\<lambda>N. N = N\<^sub>0 \<and> distinct_mset N\<^sub>0]\<^sub>a (list_mset_assn uint32_nat_assn)\<^sup>k \<rightarrow>
-      twl_array_code_ops.twl_st_assn_no_clvls N\<^sub>0\<close>
+    [\<lambda>N. N = \<A>\<^sub>i\<^sub>n \<and> distinct_mset \<A>\<^sub>i\<^sub>n]\<^sub>a (list_mset_assn uint32_nat_assn)\<^sup>k \<rightarrow>
+      twl_array_code_ops.twl_st_assn_no_clvls \<A>\<^sub>i\<^sub>n\<close>
     (is \<open>?c \<in> [?pre]\<^sub>a ?im \<rightarrow> ?f\<close>)
 proof -
-  have H: \<open>?c \<in> [\<lambda>x. x = N\<^sub>0 \<and> distinct_mset
-         N\<^sub>0]\<^sub>a (hr_comp
+  have H: \<open>?c \<in> [\<lambda>x. x = \<A>\<^sub>i\<^sub>n \<and> distinct_mset
+         \<A>\<^sub>i\<^sub>n]\<^sub>a (hr_comp
                   (list_assn uint32_assn)
                   (\<langle>uint32_nat_rel\<rangle>list_rel_mset_rel),
                  hr_comp
                   (list_assn uint32_assn)
                   (\<langle>uint32_nat_rel\<rangle>list_rel_mset_rel)) \<rightarrow> hr_comp
           (twl_array_code_ops.twl_st_int_assn
-            N\<^sub>0)
-          (twl_array_code_ops.twl_st_ref_no_clvls N\<^sub>0)\<close>
+            \<A>\<^sub>i\<^sub>n)
+          (twl_array_code_ops.twl_st_ref_no_clvls \<A>\<^sub>i\<^sub>n)\<close>
     (is \<open>_ \<in> [?pre']\<^sub>a ?im' \<rightarrow> ?f'\<close>)
-    using init_state_wl_int_hnr[FCOMP init_state_wl_int_init_state_wl, of N\<^sub>0 N\<^sub>0, simplified] .
+    using init_state_wl_int_hnr[FCOMP init_state_wl_int_init_state_wl, of \<A>\<^sub>i\<^sub>n \<A>\<^sub>i\<^sub>n, simplified] .
   have im: \<open>?im' = ?im\<close>
     by (auto simp: list_mset_assn_def list_rel_mset_rel_def hr_comp_assoc[symmetric]
         list_assn_comp list_assn_list_mset_rel_eq_list_mset_assn)
@@ -1826,7 +1826,7 @@ lemma [sepref_fr_rules]:
   by sepref_to_hoare sep_auto
 
 lemmas (in twl_array_code)init_dt_wl_code_refine'[sep_heap_rules] =
-  init_dt_wl_code.refine[of N\<^sub>0, OF twl_array_code_axioms]
+  init_dt_wl_code.refine[of \<A>\<^sub>i\<^sub>n, OF twl_array_code_axioms]
 
 lemma (in -)id_mset_list_assn_list_mset_assn:
   assumes \<open>CONSTRAINT is_pure R\<close>
@@ -1846,40 +1846,40 @@ qed
 
 lemma cdcl_twl_stgy_prog_wl_D_code_ref':
   \<open>(uncurry (\<lambda>_. cdcl_twl_stgy_prog_wl_D_code), uncurry twl_array_code.cdcl_twl_stgy_prog_wl_D)
-  \<in> [\<lambda>(N, _). N = N\<^sub>0 \<and> twl_array_code N\<^sub>0]\<^sub>a
+  \<in> [\<lambda>(N, _). N = \<A>\<^sub>i\<^sub>n \<and> twl_array_code \<A>\<^sub>i\<^sub>n]\<^sub>a
      (list_mset_assn uint32_nat_assn)\<^sup>k *\<^sub>a
-    (twl_array_code_ops.twl_st_assn N\<^sub>0)\<^sup>d \<rightarrow> twl_array_code_ops.twl_st_assn N\<^sub>0\<close>
+    (twl_array_code_ops.twl_st_assn \<A>\<^sub>i\<^sub>n)\<^sup>d \<rightarrow> twl_array_code_ops.twl_st_assn \<A>\<^sub>i\<^sub>n\<close>
   unfolding hfref_def hn_refine_def
   apply (subst in_pair_collect_simp)
   apply (intro allI impI)
   subgoal for a c
-    using cdcl_twl_stgy_prog_wl_D_code.refine[of N\<^sub>0,
+    using cdcl_twl_stgy_prog_wl_D_code.refine[of \<A>\<^sub>i\<^sub>n,
       unfolded in_pair_collect_simp hfref_def hn_refine_def PR_CONST_def,
       rule_format, of \<open>snd c\<close> \<open>snd a\<close>]
     apply (cases a)
     by (sep_auto
-      dest!: frame_rule_left[of \<open>twl_array_code_ops.twl_st_assn _ _ _\<close> _ _\<open>list_mset_assn uint32_nat_assn N\<^sub>0 (fst a)\<close>])
+      dest!: frame_rule_left[of \<open>twl_array_code_ops.twl_st_assn _ _ _\<close> _ _\<open>list_mset_assn uint32_nat_assn \<A>\<^sub>i\<^sub>n (fst a)\<close>])
   done
 
 declare cdcl_twl_stgy_prog_wl_D_code_ref'[to_hnr, OF refl, sepref_fr_rules]
 
 lemma init_dt_wl_code_refine[sepref_fr_rules]:
   \<open>(uncurry2 (\<lambda>_. init_dt_wl_code), uncurry2 (twl_array_code.init_dt_wl))
-  \<in> [\<lambda>((N, S), S'). twl_array_code N \<and> N = N\<^sub>0]\<^sub>a
+  \<in> [\<lambda>((N, S), S'). twl_array_code N \<and> N = \<A>\<^sub>i\<^sub>n]\<^sub>a
     (list_mset_assn uint32_nat_assn)\<^sup>k *\<^sub>a (list_assn (list_assn unat_lit_assn))\<^sup>d *\<^sub>a
-      (twl_array_code_ops.twl_st_assn_no_clvls N\<^sub>0)\<^sup>d \<rightarrow>
-    twl_array_code_ops.twl_st_assn_no_clvls N\<^sub>0\<close>
+      (twl_array_code_ops.twl_st_assn_no_clvls \<A>\<^sub>i\<^sub>n)\<^sup>d \<rightarrow>
+    twl_array_code_ops.twl_st_assn_no_clvls \<A>\<^sub>i\<^sub>n\<close>
   unfolding PR_CONST_def
   unfolding hfref_def hn_refine_def
   apply (subst in_pair_collect_simp)
   apply (intro allI impI)
   subgoal for a c
-    using init_dt_wl_code.refine[of N\<^sub>0,
+    using init_dt_wl_code.refine[of \<A>\<^sub>i\<^sub>n,
       unfolded in_pair_collect_simp hfref_def hn_refine_def PR_CONST_def,
       rule_format, of \<open>(snd (fst c), snd c)\<close> \<open>(snd (fst a), snd a)\<close>]
     by (cases a)
        (sep_auto dest!: frame_rule_left[of \<open>_ * twl_array_code_ops.twl_st_assn_no_clvls _ _ _\<close> _ _
-            \<open>list_mset_assn uint32_nat_assn N\<^sub>0 (fst (fst a))\<close>])
+            \<open>list_mset_assn uint32_nat_assn \<A>\<^sub>i\<^sub>n (fst (fst a))\<close>])
   done
 
 lemma pair_nat_ann_lits_assn_alt_def:
@@ -1897,8 +1897,8 @@ lemma (in twl_array_code) get_trail_wl[sepref_fr_rules]:
 
 lemma [sepref_fr_rules]:
   \<open>(return o get_trail_wl_code,
-   RETURN \<circ> get_trail_wl) \<in> [\<lambda>_. twl_array_code N\<^sub>0]\<^sub>a (twl_array_code_ops.twl_st_assn N\<^sub>0)\<^sup>d \<rightarrow> pair_nat_ann_lits_assn\<close>
-  using twl_array_code.get_trail_wl[of N\<^sub>0] by (auto simp: hfref_def)
+   RETURN \<circ> get_trail_wl) \<in> [\<lambda>_. twl_array_code \<A>\<^sub>i\<^sub>n]\<^sub>a (twl_array_code_ops.twl_st_assn \<A>\<^sub>i\<^sub>n)\<^sup>d \<rightarrow> pair_nat_ann_lits_assn\<close>
+  using twl_array_code.get_trail_wl[of \<A>\<^sub>i\<^sub>n] by (auto simp: hfref_def)
 
 lemma extract_model_of_state_alt_def:
   \<open>extract_model_of_state U = rev (map lit_of (get_trail_wl U))\<close>
@@ -1912,7 +1912,7 @@ qed
 
 sepref_definition extract_model_of_state_code
   is \<open>RETURN o extract_model_of_state\<close>
-  :: \<open>[\<lambda>_. twl_array_code N\<^sub>0]\<^sub>a (twl_array_code_ops.twl_st_assn N\<^sub>0)\<^sup>d \<rightarrow> list_assn unat_lit_assn\<close>
+  :: \<open>[\<lambda>_. twl_array_code \<A>\<^sub>i\<^sub>n]\<^sub>a (twl_array_code_ops.twl_st_assn \<A>\<^sub>i\<^sub>n)\<^sup>d \<rightarrow> list_assn unat_lit_assn\<close>
   unfolding extract_model_of_state_def map_by_foldl[symmetric]
      comp_def foldl_conv_fold foldl_conv_fold
   unfolding HOL_list.fold_custom_empty
@@ -1936,9 +1936,9 @@ sepref_definition IsaSAT_code
    option.splits[split]
   apply (rewrite at \<open>extract_atms_clss _ \<hole>\<close> op_extract_list_empty_def[symmetric])
   apply (rewrite
-      at "twl_array_code_ops.init_state_wl N\<^sub>0"
-      in "let N\<^sub>0 = _ in do {ASSERT _ ; _; let _ = \<hole> ; _}"
-      to "ASSN_ANNOT (twl_array_code_ops.twl_st_assn_no_clvls N\<^sub>0) (twl_array_code_ops.init_state_wl N\<^sub>0)"
+      at "twl_array_code_ops.init_state_wl \<A>\<^sub>i\<^sub>n"
+      in "let \<A>\<^sub>i\<^sub>n = _ in do {ASSERT _ ; _; let _ = \<hole> ; _}"
+      to "ASSN_ANNOT (twl_array_code_ops.twl_st_assn_no_clvls \<A>\<^sub>i\<^sub>n) (twl_array_code_ops.init_state_wl \<A>\<^sub>i\<^sub>n)"
     annotate_assn)
   supply [[goals_limit = 1]]
   by sepref
@@ -1979,9 +1979,9 @@ proof -
     by (subst (2) append_take_drop_id[symmetric, of \<open>tl af\<close> ag], subst mset_append)
       (auto simp: drop_Suc)
 
-  have N\<^sub>1: \<open>twl_array_code_ops.is_N\<^sub>1 (mset (extract_atms_clss CS' [])) (all_lits_of_mm (mset `# mset CS'))\<close>
+  have \<L>\<^sub>a\<^sub>l\<^sub>l: \<open>twl_array_code_ops.is_\<L>\<^sub>a\<^sub>l\<^sub>l (mset (extract_atms_clss CS' [])) (all_lits_of_mm (mset `# mset CS'))\<close>
     for CS'
-    by (auto simp add: twl_array_code_ops.is_N\<^sub>1_def twl_array_code_ops.N\<^sub>1_def
+    by (auto simp add: twl_array_code_ops.is_\<L>\<^sub>a\<^sub>l\<^sub>l_def twl_array_code_ops.\<L>\<^sub>a\<^sub>l\<^sub>l_def
       all_lits_of_mm_add_mset in_extract_atms_clssD in_extract_atms_clsD
       all_lits_of_mm_def atms_of_s_def image_image image_Un)
   have if_no_confl_ref:
@@ -2019,7 +2019,7 @@ proof -
           clauses_def get_unit_learned_def in_list_mset_rel in_list_mset_rel_mset_rel)
      subgoal
        apply (rule disjI2)
-       using N\<^sub>1 struct_invs stgy_invs corr_w UP count_dec U clss trail False
+       using \<L>\<^sub>a\<^sub>l\<^sub>l struct_invs stgy_invs corr_w UP count_dec U clss trail False
        by (cases S\<^sub>0) (clarsimp simp: twl_struct_invs_def CS twl_array_code_ops.init_state_def full_def
            get_unit_learned_def cdcl\<^sub>W_restart_mset_state)
       done
@@ -2059,19 +2059,19 @@ proof -
        (state\<^sub>W_of (twl_st_of None (st_l_of_wl None S\<^sub>0)))\<close>
       using 0 by (auto simp: S\<^sub>0 CS mset_take_mset_drop_mset' N_NP init_state.simps)
 
-    have N\<^sub>1: \<open>twl_array_code_ops.is_N\<^sub>1 (mset (extract_atms_clss CS' [])) (all_lits_of_mm (mset `# mset CS'))\<close>
-      by (auto simp add: twl_array_code_ops.is_N\<^sub>1_def twl_array_code_ops.N\<^sub>1_def
+    have \<L>\<^sub>a\<^sub>l\<^sub>l: \<open>twl_array_code_ops.is_\<L>\<^sub>a\<^sub>l\<^sub>l (mset (extract_atms_clss CS' [])) (all_lits_of_mm (mset `# mset CS'))\<close>
+      by (auto simp add: twl_array_code_ops.is_\<L>\<^sub>a\<^sub>l\<^sub>l_def twl_array_code_ops.\<L>\<^sub>a\<^sub>l\<^sub>l_def
         all_lits_of_mm_add_mset in_extract_atms_clssD in_extract_atms_clsD
         all_lits_of_mm_def atms_of_s_def image_image image_Un)
     have \<open>twl_array_code (mset (extract_atms_clss CS' []))\<close>
       unfolding twl_array_code_def
     proof
       fix L
-      assume L: \<open>L \<in># twl_array_code_ops.N\<^sub>1 (mset (extract_atms_clss CS' []))\<close>
+      assume L: \<open>L \<in># twl_array_code_ops.\<L>\<^sub>a\<^sub>l\<^sub>l (mset (extract_atms_clss CS' []))\<close>
       then obtain C where
         L: \<open>C\<in>set CS' \<and> (L \<in>set C \<or> - L \<in> set C)\<close>
         by (cases L) (auto simp: in_extract_atms_clssD upperN_def nat_of_uint32_uint32_of_nat_id
-           twl_array_code_ops.N\<^sub>1_def)
+           twl_array_code_ops.\<L>\<^sub>a\<^sub>l\<^sub>l_def)
       have \<open>\<forall>C\<in>#CS. \<forall>L\<in>#C. nat_of_lit L < upperN\<close>
         using CS_p by auto
       then have \<open>nat_of_lit L < upperN \<or> nat_of_lit (-L) < upperN\<close>
@@ -2085,7 +2085,7 @@ proof -
                      (state\<^sub>W_of (twl_st_of None (st_l_of_wl None S\<^sub>0)))
                      (state\<^sub>W_of (twl_st_of None (st_l_of_wl None T))))\<close>
       using twl_array_code.cdcl_twl_stgy_prog_wl_spec_final2[of
-              \<open>mset (extract_atms_clss CS' [])\<close> S\<^sub>0]  CS_p N\<^sub>1
+              \<open>mset (extract_atms_clss CS' [])\<close> S\<^sub>0]  CS_p \<L>\<^sub>a\<^sub>l\<^sub>l
             struct_invs stgy_invs corr_w add_invs clss 1 True by auto
 
     have \<open>twl_array_code.cdcl_twl_stgy_prog_wl_D (mset (extract_atms_clss CS' [])) S\<^sub>0
@@ -2102,11 +2102,11 @@ proof -
   unfolding twl_array_code_def
       proof
     fix L
-    assume L: \<open>L \<in># twl_array_code_ops.N\<^sub>1 (mset (extract_atms_clss CS' []))\<close>
+    assume L: \<open>L \<in># twl_array_code_ops.\<L>\<^sub>a\<^sub>l\<^sub>l (mset (extract_atms_clss CS' []))\<close>
     then obtain C where
       L: \<open>C\<in>set CS' \<and> (L \<in>set C \<or> - L \<in> set C)\<close>
       by (cases L) (auto simp: in_extract_atms_clssD upperN_def nat_of_uint32_uint32_of_nat_id
-          twl_array_code_ops.N\<^sub>1_def)
+          twl_array_code_ops.\<L>\<^sub>a\<^sub>l\<^sub>l_def)
     have \<open>nat_of_lit L < upperN \<or> nat_of_lit (-L) < upperN\<close>
       using L CS_p by auto
     then show \<open>nat_of_lit L < upperN\<close>
@@ -2123,7 +2123,7 @@ proof -
     subgoal by (auto simp: in_list_mset_rel in_list_mset_rel_mset_rel)
     subgoal by (auto simp: in_list_mset_rel in_list_mset_rel_mset_rel)
     subgoal by (auto simp: in_list_mset_rel in_list_mset_rel_mset_rel)
-    subgoal using N\<^sub>1 by simp
+    subgoal using \<L>\<^sub>a\<^sub>l\<^sub>l by simp
     done
 qed
 
@@ -2303,11 +2303,11 @@ proof -
     unfolding twl_array_code_def
   proof
     fix L
-    assume L: \<open>L \<in># twl_array_code_ops.N\<^sub>1 (mset (extract_atms_clss x []))\<close>
+    assume L: \<open>L \<in># twl_array_code_ops.\<L>\<^sub>a\<^sub>l\<^sub>l (mset (extract_atms_clss x []))\<close>
     then obtain C where
       L: \<open>C\<in>set x \<and> (L \<in>set C \<or> - L \<in> set C)\<close>
       by (cases L) (auto simp: in_extract_atms_clssD upperN_def nat_of_uint32_uint32_of_nat_id
-         twl_array_code_ops.N\<^sub>1_def)
+         twl_array_code_ops.\<L>\<^sub>a\<^sub>l\<^sub>l_def)
     have \<open>\<forall>C\<in>#y. \<forall>L\<in>#C. nat_of_lit L < upperN\<close>
       using CS_p by auto
     then have \<open>nat_of_lit L < upperN \<or> nat_of_lit (-L) < upperN\<close>
